project/out/Reactive.ml
@@ -1,0 +1,22 @@
+open Prims
+type waiting = unit
+type running = unit
+type input_event = unit
+type output_event = unit
+type state =
+  | Waiting of waiting 
+  | Running of running 
+let (uu___is_Waiting : state -> Prims.bool) =
+  fun projectee -> match projectee with | Waiting _0 -> true | uu___ -> false
+let (__proj__Waiting__item___0 : state -> waiting) =
+  fun projectee -> match projectee with | Waiting _0 -> _0
+let (uu___is_Running : state -> Prims.bool) =
+  fun projectee -> match projectee with | Running _0 -> true | uu___ -> false
+let (__proj__Running__item___0 : state -> running) =
+  fun projectee -> match projectee with | Running _0 -> _0
+let (start : state) =
+  Obj.magic (fun uu___ -> failwith "Not yet implemented:start")
+let (receive : input_event -> waiting -> (state * output_event Prims.list)) =
+  fun uu___ -> fun uu___1 -> failwith "Not yet implemented:receive"
+let (continue : running -> (state * output_event Prims.list)) =
+  fun uu___ -> failwith "Not yet implemented:continue"
