project/practice/out/Hello.ml
@@ -1,6 +1,0 @@
-open Prims
-type 'a st = Prims.int -> ('a * Prims.int)
-let (x : Prims.int) = Prims.int_zero
-let (read_and_increment : Prims.int st) =
-  fun x1 -> (x1, (x1 + Prims.int_one))
-let (incr : Prims.int -> Prims.int) = fun x1 -> x1 + Prims.int_one
