project/Top_level.fst
@@ -1,0 +1,322 @@
+module Top_level
+
+open BrowserIO
+open Assumed
+open Browser
+
+(** {3 Top-level browser functionality} *)
+
+  (** The type of a browser waiting for input. *)
+  type waiting = browser
+
+  (** The type of a browser in the middle of processing the current input. *)
+  type running = {
+    running_state: browser;
+    running_task_queue: list task;
+  }
+
+  type input_event = Io.input_event
+  type output_event = Io.output_event
+
+  (** The type of a browser state, in general. *)
+  type state =
+    | Waiting of waiting
+    | Running of running
+
+  (** The initial configuration of a browser. *)
+  let start: state =
+    Waiting ({
+      waiting_state = {
+        browser_windows = [];
+        browser_pages = [];
+        browser_nodes = [];
+        browser_environments = [];
+        browser_cookies = [];
+        browser_connections = [];
+      }
+    })
+
+  (** Handling a [User_load_in_new_win_event]. *)
+  let handle_load_in_new_win_event
+    (wo: win_opener) (wn: win_name) (u: url) (b: b)
+  : state * output_event list =
+    let (_, b', oes) = open_win wn u wo b in
+    let r = {
+      running_state = b';
+      running_task_queue = [];
+    } in
+    (Running(r), oes)
+
+  (** Handling a [User_load_in_win_event]. *)
+  let handle_load_in_win_event (wr: win_ref) (u: url) (b: b)
+  : state * output_event list =
+    assert (win_valid wr b);
+    let (b', oes) = direct_win wr u b in
+    let r = {
+      running_state = b';
+      running_task_queue = [];
+    } in
+    (Running(r), oes)
+
+  (** Handling a [User_close_win_event]. *)
+  let handle_close_win_event (wr: win_ref) (b: b)
+  : state * output_event list =
+    assert (win_valid wr b);
+    let oe = UI_win_closed_event(win_to_user_window wr b) in
+    let w' = { waiting_state = win_remove wr b } in
+    (Waiting(w'), [ oe ])
+
+  (** Handling an [User_input_text_event]. *)
+  let handle_input_text_event (wr: win_ref) (box_pos: int) (str: string) (b: b)
+  : state * output_event list =                                    
+    assert (win_valid wr b);
+    begin match textbox_handlers_in_pos wr box_pos b with
+    | None ->           
+        (Waiting({ waiting_state = b }), [])
+    | Some(dr, vs) ->
+      let task v = {
+          task_win = wr;
+          task_expr = Apply(X(R(v)), X(R(Node_value(dr))));
+        } in
+        let n' =
+          begin match node_assoc_valid dr b with
+          | Textbox_node(oeid, _, hs) -> Textbox_node(oeid, str, hs)
+          | _ -> assert false
+          end
+        in
+        let b' = node_update dr n' b in
+        let r = {
+          running_state = b';
+          running_task_queue = List.map task vs;
+        } in
+        (Running(r), [])
+    end
+
+  (** Handling a [User_click_button_event]. *)
+  let handle_click_button_event (wr: win_ref) (but_pos: int) (b: b)
+  : state * output_event list =
+    assert (win_valid wr b);
+    begin match button_handlers_in_pos wr but_pos b with
+    | None -> (Waiting({ waiting_state = b }), [])
+    | Some(dr, vs) ->
+        let task v = {
+          task_win = wr;
+          task_expr = Apply(X(R(v)), X(R(Node_value(dr))));
+        } in
+        let r = {
+          running_state = b;
+          running_task_queue = List.map task vs;
+        } in
+        (Running(r), [])
+    end
+
+  (** Return the known expressions at the head of the script queue for the page
+      in the window referenced by [wr] as browser tasks, and remove them from
+      the page's script queue. *)
+  let get_ready_exprs (wr: win_ref) (b: b)
+  : task list * b =
+    assert (win_valid wr b);
+    let task e = {
+      task_win = wr;
+      task_expr = e;
+    } in
+    let w = win_assoc_valid wr b in
+    let p = page_assoc_valid w.win_page b in
+    let (pes_ready, pes') = split_queued_exprs p.page_script_queue in
+    let p' = {
+      p with
+      page_script_queue = pes';
+    } in
+    let b' = page_update w.win_page p' b in
+    (List.map task pes_ready, b')
+
+  (** Handling a [Network_response_event]. *)
+  let handle_network_response_event
+    (Net_connection(d, n): net_connection) (resp: resp) (b: b)
+  : state * output_event list =
+    begin match net_connection_domain_nth d n b with
+    | None ->
+        (Waiting({ waiting_state = b }), [])
+    | Some((uri, dst)) ->
+        let b' = net_connection_domain_remove_nth d n b in
+        let b'1 = upd_cookies d uri resp b' in
+        begin match (dst, resp.resp_body) with
+
+        | (Xhr_dst(pr, v), Script_file(e)) when page_win pr b'1 <> None ->
+            let wr =
+              begin match page_win pr b'1 with
+              | Some(wr) -> wr
+              | None -> assert false
+              end
+            in
+            let t = {
+              task_win = wr;
+              task_expr = Apply(X(R(v)), X(R(Code_value(e))));
+            } in
+            let r = {
+              running_state = b'1;
+              running_task_queue = [ t ];
+            } in
+            (Running(r), [])
+
+        | (Doc_dst(wr), Html_file(docs)) when win_valid wr b'1 ->
+            let uw = win_to_user_window wr b'1 in
+            let w = win_assoc_valid wr b'1 in
+            let b'2 = page_remove w.win_page b'1 in
+            let (dr, node_ext) = build_node_tree (Div(None, docs)) in
+            let b'3 = {
+              b'2 with
+              browser_nodes = b'2.browser_nodes @ node_ext
+            } in
+            let (w', b'4) =
+              build_win
+                w.win_name (Http_url(d, uri)) w.win_opener (Some(dr)) b'3
+            in
+            let b'5 = win_update wr w' b'4 in
+            let rd_opt = render_page w'.win_page b'4 in
+            let oe = UI_page_loaded_event(uw, Http_url(d, uri), rd_opt) in
+            let (b'6, oes1, ts) = process_node_scripts w'.win_page dr b'5 in
+            let r = {
+              running_state = b'6;
+              running_task_queue = ts;
+            } in
+            (Running(r), [ oe ] @ oes1)
+
+        | (Doc_dst(wr), _) when win_valid wr b'1 ->
+            let uw = win_to_user_window wr b'1 in
+            let w = win_assoc_valid wr b'1 in
+            let b'3 = page_remove w.win_page b'1 in
+            let (w', b'4) =
+              build_win w.win_name (Http_url(d, uri)) w.win_opener None b'3
+            in
+            let b'5 = win_update wr w' b'4 in
+            let rd_opt = render_page w'.win_page b'5 in
+            let oe = UI_page_loaded_event(uw, Http_url(d, uri), rd_opt) in
+            (Waiting({ waiting_state = b'5 }), [ oe ])
+
+        | (Script_dst(pr, dr), Script_file(e)) when page_win pr b'1 <> None ->
+            let wr =
+              begin match page_win pr b'1 with
+              | Some(wr) -> wr
+              | None -> assert false
+              end
+            in
+            let p = page_assoc_valid pr b'1 in
+            let q = p.page_script_queue in
+            let q' =
+              let upd p =
+                begin match p with
+                | Unknown_expr(dr1) when dr1 = dr -> Known_expr(to_inner_expr e)
+                | _ -> p
+                end
+              in
+              List.map upd q
+            in
+            let p' = { p with page_script_queue = q' } in
+            let b'2 = page_update pr p' b'1 in
+            let (ts, b'3) = get_ready_exprs wr b'2 in
+            let r = {
+              running_state = b'3;
+              running_task_queue = ts;
+            } in
+            (Running(r), [])
+
+        | _ ->
+          (Waiting({ waiting_state = b'1 }), [])
+
+        end
+    end
+
+  (** Respond to an incoming event. *)
+  let receive (ie: input_event) (w: waiting)
+  : state * output_event list =
+    begin match ie with
+
+    | User_load_in_new_win_event(u) ->
+        handle_load_in_new_win_event No_opener No_name u w.waiting_state
+
+    | User_load_in_win_event(uw, u) ->
+        begin match win_from_user_window uw w.waiting_state with
+        | None -> (Waiting(w), [])
+        | Some(wr) -> handle_load_in_win_event wr u w.waiting_state
+        end
+
+    | User_link_to_new_win_event(uw, u) ->
+        let wo =
+          begin match win_from_user_window uw w.waiting_state with
+          | None -> No_opener
+          | Some(wr) -> Win_opener(wr)
+          end
+        in
+        handle_load_in_new_win_event wo No_name u w.waiting_state
+
+    | User_link_to_named_win_event(uw, str, u) ->
+        let wo =
+          begin match win_from_user_window uw w.waiting_state with
+          | None -> No_opener
+          | Some(wr) -> Win_opener(wr)
+          end
+        in
+        begin match win_from_win_name str w.waiting_state with
+        | None ->
+            handle_load_in_new_win_event wo (Str_name(str)) u w.waiting_state
+        | Some(wr) ->
+            handle_load_in_win_event wr u w.waiting_state
+        end
+
+    | User_close_win_event(uw) ->
+        begin match win_from_user_window uw w.waiting_state with
+        | None -> (Waiting(w), [])
+        | Some(wr) -> handle_close_win_event wr w.waiting_state
+        end
+
+    | User_input_text_event(User_textbox(uw, box_pos), str, _) ->
+        begin match win_from_user_window uw w.waiting_state with
+        | None -> (Waiting(w), [])
+        | Some(wr) -> handle_input_text_event wr box_pos str w.waiting_state
+        end
+
+    | User_click_button_event(User_button(uw, but_pos)) ->
+        begin match win_from_user_window uw w.waiting_state with
+        | None -> (Waiting(w), [])
+        | Some(wr) -> handle_click_button_event wr but_pos w.waiting_state
+        end
+
+    | Network_response_event(nr, resp) ->
+        handle_network_response_event nr resp w.waiting_state
+
+    end
+
+  (** Advance the browser state one step. *)
+  let continue (r: running)
+  : state * output_event list =
+    let current t = win_valid t.task_win r.running_state in
+    begin match r.running_task_queue with
+    | [] ->
+        (Waiting({ waiting_state = r.running_state}), [])
+    | t :: ts when not (current t) ->
+        let r' = { r with running_task_queue = ts } in
+        (Running(r'), [])
+    | { task_expr = X(R(Error(msg))) } :: ts ->
+        let r' = { r with running_task_queue = ts } in
+        (Running(r'), [ UI_error(msg) ])
+    | { task_expr = X(R(_)) } :: ts ->
+        let r' = { r with running_task_queue = ts } in
+        (Running(r'), [])
+    | t :: ts -> (* the task is current and not finished *)
+        let b = r.running_state in
+        let w = win_assoc_valid t.task_win b in
+        let p = page_assoc_valid w.win_page b in
+        let ctx = {
+          context_win = t.task_win;
+          context_act = p.page_environment;
+        } in
+        let (b', e', oes, ts') = step_expr ctx b t.task_expr in
+        let r' = {
+          running_state = b';
+          running_task_queue = { t with task_expr = e' } :: ts @ ts';
+        } in
+        (Running(r'), oes)
+    end
+
+
